some pipeline

compiler/src/compiler/Pipeline.v
@@ -1,4 +1,5 @@
 Require Export Coq.Lists.List.
+Require Import bedrock2.LeakageSemantics.
 Require Import Coq.ZArith.ZArith.
 Export ListNotations.
 Require Export coqutil.Decidable.
@@ -6,6 +7,7 @@ Require        compiler.ExprImp.
 Require Export compiler.FlattenExprDef.
 Require Export compiler.FlattenExpr.
 Require        compiler.FlatImp.
+Require Import compiler.FlatToRiscvDef.
 Require Export riscv.Spec.Machine.
 Require Export riscv.Platform.Run.
 Require Export riscv.Platform.RiscvMachine.
@@ -24,6 +26,7 @@ Require Import compiler.StringNameGen.
 Require Export compiler.util.Common.
 Require Export coqutil.Decidable.
 Require Export riscv.Utility.Encode.
+Require Import riscv.Spec.LeakageOfInstr.
 Require Import riscv.Spec.Decode.
 Require Export riscv.Spec.Primitives.
 Require Export riscv.Spec.MetricPrimitives.
@@ -64,10 +67,18 @@ Section WithWordAndMem.
 
   Record Lang := {
     Program: Type;
-    Valid: Program -> Prop;
-    Call(p: Program)(funcname: string)
-        (t: trace)(m: mem)(argvals: list word)(mc: MetricLog)
-        (post: trace -> mem -> list word -> MetricLog -> Prop): Prop;
+      Valid: Program -> Prop;
+      Settings: Type;
+      SettingsInhabited: Settings;
+      Leakage: Type;
+      Call(pick_sp: list Leakage -> word)(p: Program)(s: Settings)(funcname: string)
+        (k: list Leakage)(t: trace)(m: mem)(argvals: list word)(mc: MetricLog)
+        (post: list Leakage -> trace -> mem -> list word -> MetricLog -> Prop): Prop;
+      WeakenCall: forall pick_sp p s funcname k t m mc argvals (post1: _ -> _ -> _ -> _ -> _ -> Prop),
+        Call pick_sp p s funcname k t m argvals mc post1 ->
+        forall post2 : _ -> _ -> _ -> _ -> _ -> Prop,
+        (forall k' t' m' retvals mc', post1 k' t' m' retvals mc' -> post2 k' t' m' retvals mc') ->
+        Call pick_sp p s funcname k t m argvals mc post2;
   }.
 
   Record phase_correct{L1 L2: Lang}
@@ -80,12 +91,18 @@ Section WithWordAndMem.
     phase_preserves_post: forall p1 p2,
         L1.(Valid) p1 ->
         compile p1 = Success p2 ->
-        forall fname t m argvals mcH post,
-        L1.(Call) p1 fname t m argvals mcH post ->
+        forall s1 s2 fname,
+          exists pick_spH L,
+        forall pick_spL kH kL t m argvals mcH post,
+        L1.(Call) (pick_spH pick_spL kH kL) p1 s1 fname kH t m argvals mcH post ->
         forall mcL,
-        L2.(Call) p2 fname t m argvals mcL (fun t m a mcL' =>
-          exists mcH', metricsLeq (mcL' - mcL) (mcH' - mcH) /\ post t m a mcH'
-        );
+          L2.(Call) pick_spL p2 s2 fname kL t m argvals mcL
+               (fun kL' t m a mcL' =>
+                  exists mcH' kH' kH'',
+                    post kH' t m a mcH' /\
+                      kH' = kH'' ++ kH /\
+                      kL' = L kH'' ++ kL /\
+                      metricsLeq (mcL' - mcL) (mcH' - mcH));
   }.
 
   Arguments phase_correct : clear implicits.
@@ -110,28 +127,37 @@ Section WithWordAndMem.
   Proof.
     unfold compose_phases.
     intros [V12 C12] [V23 C23].
-    split; intros; fwd; [eauto|].
-    erewrite f_equal; [eauto|].
-    post_ext.
-    split; [|destruct 1 as (?&?&?&?&?)]; eauto with metric_arith.
+    split; intros; fwd; eauto.
+    specialize (V12 p1 a E H).
+    specialize (C23 a p2 V12 H0 L2.(SettingsInhabited) s2 fname).
+    specialize (C12 p1 a H E s1 L2.(SettingsInhabited) fname).
+    destruct C12 as [f12 [nps12 C12] ]. destruct C23 as [f23 [nps23 C23] ].
+    exists (fun pick_sp3 k1 k3 => f12 (f23 pick_sp3 nil k3) k1 nil).
+    exists (fun k1 => nps23 (nps12 k1)).
+    intros. eapply L3.(WeakenCall).
+    { eapply C23. eapply C12. eapply H1. }
+    simpl. intros. fwd. do 3 eexists. split; [eassumption|]. split; [reflexivity|].
+    split; [|eauto with metric_arith].
+    f_equal. f_equal. apply app_inv_tail in H2p0p2. assumption.
+    Unshelve. all: auto.
   Qed.
 
   Section WithMoreParams.
     Context {Zlocals: map.map Z word}
             {string_keyed_map: forall T: Type, map.map string T} (* abstract T for better reusability *)
-            {ext_spec: ExtSpec}
+            {ext_spec: LeakageSemantics.ExtSpec}
             {word_ok : word.ok word}
             {mem_ok: map.ok mem}
             {string_keyed_map_ok: forall T, map.ok (string_keyed_map T)}
             {Zlocals_ok: map.ok Zlocals}.
 
-    Context {ext_spec_ok : Semantics.ext_spec.ok ext_spec}.
+    Context {ext_spec_ok : LeakageSemantics.ext_spec.ok ext_spec}.
 
     (* for riscv phase: *)
     Context {Registers: map.map Z word}.
     Context {M: Type -> Type}.
     Context {MM: Monad M}.
-    Context {RVM: RiscvProgram M word}.
+    Context {RVM: RiscvProgramWithLeakage M word}.
     Context {PRParams: PrimitivesParams M MetricRiscvMachine}.
     Context {word_riscv_ok: RiscvWordProperties.word.riscv_ok word}.
     Context {Registers_ok: map.ok Registers}.
@@ -140,8 +166,10 @@ Section WithWordAndMem.
     Context {BWM: bitwidth_iset width iset}.
     Context (compile_ext_call : string_keyed_map Z -> Z -> Z -> FlatImp.stmt Z ->
                                 list Instruction).
+    Context (leak_ext_call : string_keyed_map Z -> Z -> Z -> FlatImp.stmt Z ->
+                             list word -> list LeakageEvent).
     Context (compile_ext_call_correct: forall resvars extcall argvars,
-                compiles_FlatToRiscv_correctly compile_ext_call compile_ext_call
+                compiles_FlatToRiscv_correctly compile_ext_call leak_ext_call compile_ext_call
                                                (FlatImp.SInteract resvars extcall argvars)).
     Context (compile_ext_call_length_ignores_positions:
                forall stackoffset posmap1 posmap2 c pos1 pos2,
@@ -155,50 +183,109 @@ Section WithWordAndMem.
 
     Definition locals_based_call_spec{Var Cmd: Type}{locals: map.map Var word}
                {string_keyed_map: forall T: Type, map.map string T}
-               (Exec: string_keyed_map (list Var * list Var * Cmd)%type ->
-                      Cmd -> trace -> mem -> locals -> MetricLog ->
-                      (trace -> mem -> locals -> MetricLog -> Prop) -> Prop)
-               (e: string_keyed_map (list Var * list Var * Cmd)%type)(f: string)
-               (t: trace)(m: mem)(argvals: list word)(mc: MetricLog)
-               (post: trace -> mem -> list word -> MetricLog -> Prop): Prop :=
+               (Exec: PickSp -> string_keyed_map (list Var * list Var * Cmd)%type ->
+                      Cmd -> leakage -> trace -> mem -> locals -> MetricLog ->
+                      (leakage -> trace -> mem -> locals -> MetricLog -> Prop) -> Prop)
+               (pick_sp: PickSp)
+               (e: string_keyed_map (list Var * list Var * Cmd)%type)(s : unit) (f: string)
+               (k: leakage)(t: trace)(m: mem)(argvals: list word)(mc: MetricLog)
+               (post: leakage -> trace -> mem -> list word -> MetricLog -> Prop): Prop :=
       exists argnames retnames fbody l,
         map.get e f = Some (argnames, retnames, fbody) /\
         map.of_list_zip argnames argvals = Some l /\
-        Exec e fbody t m l (cost_spill_spec mc) (fun t' m' l' mc' =>
+        Exec pick_sp e fbody k t m l (cost_spill_spec mc) (fun k' t' m' l' mc' =>
                        exists retvals, map.getmany_of_list l' retnames = Some retvals /\
-                                       post t' m' retvals mc').
+                                       post k' t' m' retvals mc').
 
     Definition locals_based_call_spec_spilled{Var Cmd: Type}{locals: map.map Var word}
                {string_keyed_map: forall T: Type, map.map string T}
-               (Exec: string_keyed_map (list Var * list Var * Cmd)%type ->
-                      Cmd -> trace -> mem -> locals -> MetricLog ->
-                      (trace -> mem -> locals -> MetricLog -> Prop) -> Prop)
-               (e: string_keyed_map (list Var * list Var * Cmd)%type)(f: string)
-               (t: trace)(m: mem)(argvals: list word)(mc: MetricLog)
-               (post: trace -> mem -> list word -> MetricLog -> Prop): Prop :=
+               (Exec: PickSp -> string_keyed_map (list Var * list Var * Cmd)%type ->
+                      Cmd -> leakage -> trace -> mem -> locals -> MetricLog ->
+                      (leakage -> trace -> mem -> locals -> MetricLog -> Prop) -> Prop)
+               (pick_sp : PickSp)
+               (e: string_keyed_map (list Var * list Var * Cmd)%type)(s : unit)(f: string)
+               (k: leakage) (t: trace)(m: mem)(argvals: list word)(mc: MetricLog)
+               (post: leakage -> trace -> mem -> list word -> MetricLog -> Prop): Prop :=
       exists argnames retnames fbody l,
         map.get e f = Some (argnames, retnames, fbody) /\
         map.of_list_zip argnames argvals = Some l /\
-        Exec e fbody t m l mc (fun t' m' l' mc' =>
+        Exec pick_sp e fbody k t m l mc (fun k' t' m' l' mc' =>
                        exists retvals, map.getmany_of_list l' retnames = Some retvals /\
-                                       post t' m' retvals mc').
+                                       post k' t' m' retvals mc').
 
+    Lemma thing_locals_based_call_spec_weaken{Var Cmd: Type}{locals: map.map Var word}
+      {string_keyed_map_: forall T: Type, map.map string T}
+      thing :
+      forall
+      (Exec: PickSp -> string_keyed_map_ (list Var * list Var * Cmd)%type ->
+             Cmd -> leakage -> trace -> mem -> locals -> MetricLog ->
+             (leakage -> trace -> mem -> locals -> MetricLog -> Prop) -> Prop),
+      (forall pick_sp e c k t m l mc (post1: _ -> _ -> _ -> _ -> _ -> Prop),
+          Exec pick_sp e c k (t : trace) m (l : map.rep) (mc : MetricLog) post1 ->
+          forall (post2 : _ -> _ -> _ -> _ -> _ -> Prop),
+            (forall k' t' m' l' mc', post1 k' t' m' l' mc' -> post2 k' t' m' l' mc') ->
+            Exec pick_sp e c k t m l mc post2) ->
+      forall
+        (pick_sp : PickSp)(e: string_keyed_map_ (list Var * list Var * Cmd)%type)(s : unit)(f: string)
+        (k: leakage)(t: trace)(m: mem)(argvals: list word)(mc: MetricLog)
+        (post1: leakage -> trace -> mem -> list word -> MetricLog -> Prop),
+        (match thing with | true => locals_based_call_spec | false => locals_based_call_spec_spilled end) Exec pick_sp e s f k t m argvals mc post1 ->
+        forall (post2 : _ -> _ -> _ -> _ -> _ -> Prop),
+          (forall k' t' m' retvals mc', post1 k' t' m' retvals mc' -> post2 k' t' m' retvals mc') ->
+          (match thing with | true => locals_based_call_spec | false => locals_based_call_spec_spilled end) Exec pick_sp e s f k t m argvals mc post2.
+    Proof.
+      destruct thing; simpl.
+      - intros. cbv [locals_based_call_spec] in *.
+        destruct H0 as (argnames & retnames & fbody & l & H2 & H3 & H4).
+        exists argnames, retnames, fbody, l. intuition eauto.
+        eapply H. 1: apply H4. simpl. intros.
+        destruct H0 as [retvals [H5 H6] ]. exists retvals. eauto.
+      - intros. cbv [locals_based_call_spec_spilled] in *.
+        destruct H0 as (argnames & retnames & fbody & l & H2 & H3 & H4).
+        exists argnames, retnames, fbody, l. intuition eauto.
+        eapply H. 1: apply H4. simpl. intros.
+        destruct H0 as [retvals [H5 H6] ]. exists retvals. eauto.
+    Qed.
+
+    Definition locals_based_call_spec_weaken {Var Cmd: Type}{locals: map.map Var word}
+      := ltac:(let t := eval compute in (thing_locals_based_call_spec_weaken (Var := Var) (Cmd := Cmd) true) in exact t).
+    Check locals_based_call_spec_weaken.
+
+    Definition locals_based_call_spec_spilled_weaken {Var Cmd: Type}{locals: map.map Var word}
+      := thing_locals_based_call_spec_weaken (Var := Var) (Cmd := Cmd) false.
+    
     Definition ParamsNoDup{Var: Type}: (list Var * list Var * FlatImp.stmt Var) -> Prop :=
       fun '(argnames, retnames, body) => NoDup argnames /\ NoDup retnames.
 
-    Definition SrcLang: Lang := {|
+    Check @MetricLeakageSemantics.exec. Print mem.
+    Check locals_based_call_spec_weaken. Print env.
+    Print string_keyed_map.
+
+    Definition SrcLang: Lang. refine ({|
       Program := Semantics.env;
       Valid := map.forall_values ExprImp.valid_fun;
-      Call := locals_based_call_spec MetricSemantics.exec;
-    |}.
-    (* |                 *)
+      Call := locals_based_call_spec (fun pick_sp e => @MetricLeakageSemantics.exec _ _ _ _ _ _ _ pick_sp);
+      SettingsInhabited := tt;
+                                       |}).
+      intros. Fail apply @locals_based_call_spec_weaken. (* why :( *)
+      cbv [locals_based_call_spec] in *. fwd. do 4 eexists. intuition eauto.
+      eapply MetricLeakageSemantics.exec.weaken; eauto. simpl. intros. fwd.
+      intuition eauto. Unshelve. assumption.
+    Defined.
+     (* |                 *)
     (* | FlattenExpr     *)
-    (* V                 *)
-    Definition FlatWithStrVars: Lang := {|
-      Program := string_keyed_map (list string * list string * FlatImp.stmt string);
-      Valid := map.forall_values ParamsNoDup;
-      Call := locals_based_call_spec (FlatImp.exec PreSpill isRegStr);
-    |}.
+    (* V                 *) Check FlatImp.exec.
+    Definition FlatWithStrVars: Lang.
+      refine ({|
+                 Program := string_keyed_map (list string * list string * FlatImp.stmt string);
+                 Valid := map.forall_values ParamsNoDup;
+                 Call := locals_based_call_spec (fun pick_sp => FlatImp.exec (pick_sp := pick_sp) PreSpill isRegStr);
+               |}).
+      1: exact tt. intros.
+      cbv [locals_based_call_spec] in *. fwd. do 4 eexists. intuition eauto.
+      eapply FlatImp.exec.weaken; eauto. simpl. intros. fwd.
+      intuition eauto.
+    Defined.                         
 
     (* |                 *)
     (* | UseImmediate    *)
@@ -213,31 +300,72 @@ Section WithWordAndMem.
     (* |                 *)
     (* | RegAlloc        *)
     (* V                 *)
-    Definition FlatWithZVars: Lang := {|
-      Program := string_keyed_map (list Z * list Z * FlatImp.stmt Z);
-      Valid := map.forall_values ParamsNoDup;
-      Call := locals_based_call_spec (FlatImp.exec PreSpill isRegZ);
-    |}.
+    Definition FlatWithZVars: Lang.
+      refine ({|
+                 Program := string_keyed_map (list Z * list Z * FlatImp.stmt Z);
+                 Valid := map.forall_values ParamsNoDup;
+                 Call := locals_based_call_spec (fun pick_sp => FlatImp.exec (pick_sp := pick_sp) PreSpill isRegZ);
+               |}).
+      1: exact tt. intros.
+      cbv [locals_based_call_spec] in *. fwd. do 4 eexists. intuition eauto.
+      eapply FlatImp.exec.weaken; eauto. simpl. intros. fwd.
+      intuition eauto.
+    Defined.
+                                    
     (* |                 *)
     (* | Spilling        *)
     (* V                 *)
-    Definition FlatWithRegs: Lang := {|
-      Program := string_keyed_map (list Z * list Z * FlatImp.stmt Z);
-      Valid := map.forall_values FlatToRiscvDef.valid_FlatImp_fun;
-      Call := locals_based_call_spec_spilled (FlatImp.exec PostSpill isRegZ);
-    |}.
+    Definition FlatWithRegs: Lang.
+      refine ({|
+                 Program := string_keyed_map (list Z * list Z * FlatImp.stmt Z);
+                 Valid := map.forall_values FlatToRiscvDef.valid_FlatImp_fun;
+                 Call := locals_based_call_spec_spilled (fun pick_sp => FlatImp.exec (pick_sp := pick_sp) PostSpill isRegZ);
+               |}).
+      1: exact tt. intros.
+      cbv [locals_based_call_spec_spilled] in *. fwd. do 4 eexists. intuition eauto.
+      eapply FlatImp.exec.weaken; eauto. simpl. intros. fwd.
+      intuition eauto.
+    Defined.
+
+    (*Lemma riscv_call_weaken :
+      forall (pick_sp: list LeakageEvent -> word) (p : list Instruction * string_keyed_map Z * Z)
+             (s : word * word) (funcname : string) (k : list LeakageEvent)
+             (t : trace) (m : mem) (argvals : list word)
+             (post1 : list LeakageEvent -> trace -> mem -> list word -> Prop),
+        (fun _ => riscv_call p s funcname k t m argvals post1) pick_sp ->
+        forall
+          post2 : list LeakageEvent -> trace -> mem -> list word -> Prop,
+          (forall (k' : list LeakageEvent) (t' : io_trace) 
+                  (m' : mem) (retvals : list word),
+              post1 k' t' m' retvals -> post2 k' t' m' retvals) ->
+          (fun _ => riscv_call p s funcname k t m argvals post2) pick_sp.
+    Proof.
+      intros. cbv [riscv_call] in *. destruct p. destruct p. destruct s.
+      destruct H as [f_rel_pos H]. exists f_rel_pos. intuition eauto.
+      cbv [runsTo]. eapply runsToNonDet.runsTo_weaken. 1: eapply H2.
+      all: try eassumption. simpl. intros. fwd. exists mH', retvals.
+      intuition eauto.
+    Qed.*)
     (* |                 *)
     (* | FlatToRiscv     *)
     (* V                 *)
-    Definition RiscvLang: Lang := {|
-      Program :=
-        list Instruction *      (* <- code of all functions concatenated       *)
-        string_keyed_map Z *    (* <- position (offset) for each function      *)
-        Z;                      (* <- required stack space in XLEN-bit words   *)
-      (* bounds in instructions are checked by `ptsto_instr` *)
-      Valid '(insts, finfo, req_stack_size) := True;
-      Call := riscv_call;
-    |}.
+    Definition RiscvLang: Lang.
+      refine ({|
+                 Program :=
+                   list Instruction *      (* <- code of all functions concatenated       *)
+                     string_keyed_map Z *    (* <- position (offset) for each function      *)
+                     Z;                      (* <- required stack space in XLEN-bit words   *)
+                 (* bounds in instructions are checked by `ptsto_instr` *)
+                 Valid '(insts, finfo, req_stack_size) := True;
+                 Call := (fun _ => riscv_call);
+               |}).
+      1: exact (word.of_Z 0, word.of_Z 0, word.of_Z 0). intros.
+      intros. cbv [riscv_call] in *. destruct p. destruct p. destruct s as [ [? ?] ?].
+      destruct H as [f_rel_pos H]. exists f_rel_pos. intuition eauto.
+      cbv [runsTo]. eapply runsToNonDet.runsTo_weaken. 1: eapply H2.
+      all: try eassumption. simpl. intros. fwd. do 3 eexists.
+      intuition eauto.
+    Defined.
 
     Lemma flatten_functions_NoDup: forall funs funs',
         (forall f argnames retnames body,
@@ -262,7 +390,9 @@ Section WithWordAndMem.
         unfold valid_fun in *.
         intros. specialize H0 with (1 := H2). simpl in H0. eapply H0.
       }
-      unfold locals_based_call_spec. intros. fwd.
+      unfold locals_based_call_spec. intros.
+      exists (fun pick_spL kH kL k => pick_spL ((rev (skipn (length kH) (rev k)) ++ kL))).
+      exists (fun k => k). intros. fwd.
       pose proof H0 as GF.
       unfold flatten_functions in GF.
       eapply map.try_map_values_fw in GF. 2: eassumption.
@@ -272,7 +402,14 @@ Section WithWordAndMem.
       eapply FlatImp.exec.weaken.
       - eapply flattenStmt_correct_aux.
         + eassumption.
-        + eauto.
+        + eapply MetricLeakageSemantics.exec.exec_ext. 
+          1: eapply MetricLeakageSemantics.exec.exec_to_other_trace.
+          1: eapply H1p2.
+          intros. simpl. simpl_rev. rewrite List.skipn_app_r.
+          2: rewrite length_rev; reflexivity.
+          simpl_rev. rewrite List.skipn_app_r.
+          2: rewrite length_rev; reflexivity.
+          rewrite rev_involutive. reflexivity.
         + reflexivity.
         + match goal with
           | |- ?p = _ => rewrite (surjective_pairing p)
@@ -293,7 +430,8 @@ Section WithWordAndMem.
         + eapply @freshNameGenState_disjoint_fbody.
       - simpl. intros. fwd. eexists. split.
         + eauto using map.getmany_of_list_extends.
-        + eexists. split; [|eassumption]. unfold cost_spill_spec in *; solve_MetricLog.
+        + do 3 eexists. split; [eassumption|]. ssplit; [align_trace|align_trace|].
+          unfold cost_spill_spec in *; solve_MetricLog.
     Qed.
 
     Lemma useimmediate_functions_NoDup: forall funs funs',
